scheduler/example/NDSMainA.v
@@ -1,24 +1,37 @@
 Require Import CRIS.
 Require Import CallFilter.
+Require Import SchHeader SchA.
+Require Import RRSHeader RRSA.
+Require Import RRSNodeHeader RRSNodeA.
+Require Import MemHeader MemA.
 Require Import NDSMainI.
 Set Implicit Arguments.
 
 Module NDSMainA. Section NDSMainA.
   Context `{_crisG: !crisG Γ Σ α β τ _S _I, _concG: !concG}.
   Context `{_schG: !SchA.newschG}.
+  Context `{_rrsG: !RRSA.rrsG}.
+  Context `{_memG: !MemA.memG}.
+  Context `{_nodeG: !RRSNodeA.nodeG}.
 
-  Definition fnsems : fnsems_type :=
-    [(None, (true, wmask_all, [], (None, NDSMainI.main)))].
+  Definition main_spec E : fspec :=
+    fspec_winv E
+      (fspec_simple (λ (_: unit),
+           (λ varg, ⌜varg = tt↑⌝ ∗ RRSAS.InitRRS ∗ RRSNodeAS.full_val (Vint 0),
+           λ vret, ⌜vret = tt↑⌝)%I)).
 
-  Program Definition smod: SMod.t :=
+  Definition fnsems E : fnsems_type :=
+    [(None, (true, wmask_all, [], (Some (main_spec E), NDSMainI.main)))].
+
+  Program Definition smod E: SMod.t :=
     {|
       SMod.scopes := [];
-      SMod.fnsems := fnsems;
+      SMod.fnsems := fnsems E;
       SMod.initial_st := [];
     |}.
   Solve All Obligations with prove_scope.
   Next Obligation. prove_nodup. Qed.
 
-  Definition t sp := Seal.sealing CRIS (SMod.to_mod sp smod).
+  Definition t E sp := Seal.sealing CRIS (SMod.to_mod sp (smod E)).
 
 End NDSMainA. End NDSMainA.
