scheduler/example/NDSMainIAproof.v
@@ -1,0 +1,92 @@
+Require Import CRIS.
+Require Import SchHeader SchA SchTactics.
+Require Import RRSHeader RRSA.
+Require Import MemHeader MemA.
+Require Import RRSNodeHeader RRSNodeI RRSNodeA.
+Require Import NDSMainI NDSMainA.
+Require Import ltac2_lib.
+
+Module NDSMainIA. Section NDSMainIA.
+  Import NDSMainA.
+  Context `{_crisG: !crisG Γ Σ α β τ _S _I, _concG: !concG}.
+  Context `{_schG: !SchA.newschG}.
+  Context `{_rrsG: !RRSA.rrsG}.
+  Context `{_memG: !MemA.memG}.
+  Context `{_nodeG: !RRSNodeA.nodeG}.
+
+  Context (E: coPset).
+  Context (sp: sp_type).
+  Context (sp_sch_user sp_user: spl_type).
+  Context (Hschglob: sp_incl sp_sch_user sp).
+  Context (Hschrrs: spl_sub sp_user sp_sch_user).
+  Context (Hsch: sp_incl (SchA.sp sp_sch_user E) sp).
+  Context (Hrrs: spl_sub (RRSAS.sp sp_user E) sp_sch_user).
+  Context (Hnode: spl_sub (RRSNodeAS.sp E) sp_user).
+
+  Local Definition MA := (NDSMainA.t E sp).
+  Local Definition MI := (NDSMainI.t).
+
+  Lemma simF_main : ISim.sim_fun open MA MI emp%I IstTrue None.
+  Proof using Hschglob Hschrrs Hsch Hrrs Hnode.
+    init_simF.
+
+    steps_l. iDestruct "ASM" as "((-> & I & F) & ->)".
+    force_l (λ svarg sarg, ⌜svarg = RRSNodeHdr.f_main↑↑ ∧ svarg = sarg⌝ ∗ RRSAS.InitRRS ∗ RRSNodeAS.full_val (Vint 0),
+              λ svret sret, existT 0 (SL.pure False))%I.
+    forces_l. iSplitL "I F".
+    { iExists _. iSplit; eauto.  do 3 iExists _. iSplit; eauto; cycle 1.
+      { iFrame. iSplit; eauto. }
+      { iPureIntro. esplits; eauto. r. exists (RRSAS.init_spec sp_user E). esplits; eauto.
+        { eapply Hrrs. rewrite /RRSAS.sp. unseal CRIS. ss. }
+        econs. ss. Unshelve.
+        2:{ ss. eexact (x1.1, x1.2, (λ (svarg sarg : SAny.t), ⌜svarg = sarg ∧ sarg = tt↑↑⌝ ∗ RRSNodeAS.full_val (Vint 0), existT 0 (RRSNodeAS.x_value_tid 0))%I). }
+        esplits; eauto.
+        { destruct x1 as [mtid stid]. iIntros (??) "(WI & % & % & tidF & % & % & % & I & F)"; des; subst; hss.
+          rewrite /RRSAS.init_spec /fspec_sch /fspec_winv /precond /=.
+          iFrame. iModIntro. iExists _. iSplit; eauto. iExists _. iPureIntro. esplits; eauto.
+          rr. exists (RRSNodeAS.f_main_spec E). esplits; eauto.
+          { eapply Hnode. rewrite /RRSNodeAS.sp. unseal CRIS. ss. }
+          ii; ss. destruct x1 as [[mtid' stid'] ssch']. exists (stid', ssch'). esplits; eauto.
+          { iIntros (??) "(WI & % & % & tidF & RRI & % & % & % & % & F)"; des; subst; hss.
+            iFrame. eauto. }
+          { iIntros (??) "(WI & (% & tidF) & %)"; des; subst; hss.
+            rewrite /fspec_winv /fspec_virtual /postcond. iFrame.
+            iModIntro. iExists (tt↑↑). iSplit; eauto. }
+        }
+        { iIntros (??) "(WI & tidF & % & % & X)". ss. }
+      }
+    }
+
+    steps_r; steps_l; hss. call "IST". steps_l.
+    iDestruct "ASM" as "(% & % & % & % & Join)"; des; subst; hss.
+    forces_l. iSplitR; eauto.
+    steps_r. step. iFrame; eauto.
+  Qed.
+
+  Lemma sim : ISim.t open MA MI emp%I IstTrue.
+  Proof using Hschglob Hschrrs Hsch Hrrs Hnode.
+    init_sim. eapply simF_main.
+  Qed.
+
+End NDSMainIA. End NDSMainIA.
+
+Section ctxr.
+  Context `{_crisG: !crisG Γ Σ α β τ _S _I, _concG: !concG}.
+  Context `{_schG: !SchA.newschG}.
+  Context `{_rrsG: !RRSA.rrsG}.
+  Context `{_memG: !MemA.memG}.
+  Context `{_nodeG: !RRSNodeA.nodeG}.
+
+  Lemma ctxr E sp sp_sch_user sp_user
+    (Hschglob: sp_incl sp_sch_user sp)
+    (Hschrrs: spl_sub sp_user sp_sch_user)
+    (Hsch: sp_incl (SchA.sp sp_sch_user E) sp)
+    (Hrrs: spl_sub (RRSAS.sp sp_user E) sp_sch_user)
+    (Hnode: spl_sub (RRSNodeAS.sp E) sp_user) :
+    ctx_refines
+      (NDSMainA.t E sp, emp%I)
+      (NDSMainI.t     , emp%I).
+  Proof using. eapply main_adequacy, (NDSMainIA.sim E sp sp_sch_user sp_user); eauto. Qed.
+
+End ctxr.
+
